maybe stack_cont is not necessary

theories/stack.v
@@ -7,19 +7,9 @@ From iris.heap_lang Require Import proofmode notation.
 From iris_examples Require Import treiber2.
 From play Require Import history.
 
-Section stack_stuff.
-  Typeclasses Transparent is_stack stack_cont.
-  Context `{!heapG Σ, !stackG Σ}.
-  Global Instance is_stack_persistent N l γ : Persistent (is_stack N l γ).
-  Proof. apply _. Qed.
-  Global Instance stack_cont_laterable l γ : Laterable (stack_cont l γ).
-  Proof. apply _. Qed.
-  Global Instance stack_cont_timeless l γ : Timeless (stack_cont l γ).
-  Proof. apply _. Qed.
-  Global Instance to_val_inj : Inj (=) (=) to_val.
-  Proof. intros l1 l2 H. case l1, l2; try done. inversion H. reflexivity. Qed.
-  Typeclasses Opaque is_stack stack_cont.
-End stack_stuff.
+Instance to_val_inj : Inj (=) (=) to_val.
+Proof. intros l1 l2 H. case l1, l2; try done. by inversion H. Qed.
+
 Local Hint Extern 0 (environments.envs_entails _ (phys_stack _ [])) => iExists None : core.
 Local Hint Extern 0 (environments.envs_entails _ (phys_stack _ (_ :: _))) => iExists (Some _) : core.
 Local Hint Extern 10 (environments.envs_entails _ (phys_stack _ _)) => unfold phys_stack : core.
@@ -27,13 +17,13 @@ Local Hint Extern 0 (environments.envs_entails _ (phys_list None [])) => simpl :
 Local Hint Extern 0 (environments.envs_entails _ (phys_list (Some _) (_ :: _))) => simpl : core.
 
 (* NOTE: iFrame may fail for Opaque definitions  *)
-Typeclasses Transparent hist hist_snap stack_cont.
+Typeclasses Transparent hist hist_snap.
 Section spec.
   Inductive stack_op := Push of val | Pop of val.
   Canonical Structure stack_opO := leibnizO stack_op.
   Definition Hist := @Hist stack_opO.
 
-  Context `{!heapG Σ, !stackG Σ, !@histG stack_opO Σ} (N : namespace).
+  Context `{!heapG Σ, !@histG stack_opO Σ} (N : namespace).
 
   Definition stack_hist_entry_le : relation (nat * excl stack_op) :=
     λ (x y : (nat * excl stack_op)), x.1 <= y.1.
@@ -54,6 +44,8 @@ Section spec.
 
   Definition stack_hist_cont (hs : Hist) : option (list val) :=
     stack_hist_cont_aux [] $ merge_sort stack_hist_entry_le $ gmap_to_list hs .
+
+  (* TODO: use relation? *)
 
   (* Fixpoint stack_hist_cont_aux (hs : Hist) s l : option (list val) :=
        match l with
@@ -91,63 +83,51 @@ Section spec.
   Proof.
   Admitted.
 
-  (* TODO: need to track last timestamp? *)
-  Definition stack_hist γs γh l :=
-    inv N (∃ hs t xs, phys_stack l xs ∗ own γs (● Excl' xs) ∗
-                      hist γh hs t ∗ ⌜stack_hist_cont hs = Some xs⌝).
-
-  (* impossible? stack_hist γs γh l -∗ is_stack γs l. *)
-
-  (* TODO: what rel for stack_cont and hist_snap? *)
-  Definition stack_hist_snap γs γh q xs hs : iProp Σ :=
-    stack_cont γs xs ∗
-    hist_snap γh q hs ∗
-    ⌜∃ hsM tM, hs ≼ hsM ∧ hist_gapless tM hsM ∧ stack_hist_cont hsM = Some xs⌝.
+  (* NOTE: the client with full ownership should be able to assemble the history
+     into a valid stack representation *)
+  Definition stack_hist γh l :=
+    inv N (∃ hs t xs, phys_stack l xs ∗ hist γh hs t ∗ ⌜stack_hist_cont hs = Some xs⌝).
 
   Lemma new_stack_spec_hist :
     {{{ True }}}
       new_stack #()
-    {{{ l γs γh, RET #l; stack_hist γs γh l ∗ stack_hist_snap γs γh 1 [] ε }}}.
+    {{{ l γh, RET #l; stack_hist γh l ∗ hist_snap γh 1 ε }}}.
   Proof.
     iIntros (Φ) "_ HΦ".
     iApply wp_fupd.
     wp_lam. wp_alloc l as "Hl".
-    iMod (own_alloc (● (Excl' []) ⋅ ◯ (Excl' []))) as (γs) "[Hs● Hs◯]";
-      first by apply auth_both_valid.
     iMod hist_alloc as (γh) "[Hh● Hh◯]".
-    iMod (inv_alloc N _
-                    (∃ (hs : Hist) t xs,
-                        phys_stack l xs ∗ own γs (● Excl' xs) ∗
-                        hist γh hs t ∗ ⌜stack_hist_cont hs = Some xs⌝)
-            with "[Hl Hs● Hh●]").
+    iMod (inv_alloc
+            N _ (∃ (hs : Hist) t xs,
+                    phys_stack l xs ∗ hist γh hs t ∗ ⌜stack_hist_cont hs = Some xs⌝)
+            with "[Hl Hh●]").
     { iNext; iExists ε, O, []. iFrame. iSplitL "Hl". eauto with iFrame.
       iPureIntro. apply stack_hist_cont_empty. }
-    iModIntro. iApply "HΦ". iFrame. iPureIntro. by exists ε, O.
+    iModIntro. iApply "HΦ". iFrame.
   Qed.
 
 
-  Lemma push_stack_spec_hist (l : loc) (γs γh : gname) (v : val) :
-    stack_hist γs γh l -∗
-    <<< ∀ xs q hs, stack_hist_snap γs γh q xs hs >>>
+  Lemma push_stack_spec_hist (l : loc) (γh : gname) (v : val) :
+    stack_hist γh l -∗
+    <<< ∀ q hs, hist_snap γh q hs >>>
       push_stack v #l @ ⊤ ∖ ↑N
-    <<< ∃ (t:nat), stack_hist_snap γs γh q (v::xs) (<[t := Excl (Push v)]> hs) ∗
+    <<< ∃ (t:nat), hist_snap γh q (<[t := Excl (Push v)]> hs) ∗
                  ⌜∀ (t':nat), t' ∈ (dom (gset nat) hs) → t' < t⌝,
         RET #() >>>.
   Proof.
     iIntros "#SH" (Φ) "AU". iLöb as "IH".
     wp_lam; wp_let; wp_bind (! _)%E.
-    iInv "SH" as (hsM tM xs) ">(HPhys & Hs● & Hh● & %)". rename H0 into Hcont.
+    iInv "SH" as (hsM tM xs) ">(HPhys & Hh● & %)". rename H0 into Hcont.
     iDestruct "HPhys" as (w) "[Hl HPhys]".
     wp_load. iModIntro. iSplitR "AU"; first by eauto 10 with iFrame.
     clear Hcont hsM tM xs.
 
     wp_alloc r as "Hr". wp_inj. wp_bind (CmpXchg _ _ _)%E.
-    iInv "SH" as (hsM tM ys) ">(HPhys & Hs● & Hh● & %)". rename H0 into Hcont.
+    iInv "SH" as (hsM tM xs) ">(HPhys & Hh● & %)". rename H0 into Hcont.
     iDestruct "HPhys" as (u) "[Hl HPhys]".
     destruct (decide (u = w)) as [[= ->]|NE].
     - wp_cmpxchg_suc; first by case w; left. (* TODO: solve_vals_compare_safe doesn't work *)
-      iMod "AU" as (zs q hs) "[(Hs◯ & Hh◯ & %) [_ HClose]]". rename H0 into Hcont_frag.
-      iDestruct (auth_agree with "Hs● Hs◯") as %->.
+      iMod "AU" as (q hs) "[Hh◯ [_ CloseAU]]".
 
       (* TODO: just to extract pure stuff. simpler solution? *)
       iDestruct "Hh●" as "[Hh● Hg]". iDestruct "Hg" as %Hg.
@@ -155,63 +135,61 @@ Section spec.
       iDestruct (own_valid_2 with "Hh● Hh◯") as %Hincl%frac_auth_included_total.
       iCombine "Hh●" "Hg" as "Hh●". iClear "Hg".
 
-      iMod (auth_update γs (v::zs) with "Hs● Hs◯") as "[Hs● Hs◯]".
       iMod (hist_update γh q hsM hs tM (Push v) with "Hh● Hh◯") as "[Hh● Hh◯]".
-      rewrite /stack_hist_snap /hist /hist_snap.
       iDestruct "Hh●" as "[Hh● %]". rename H0 into Hg'.
       set hsM' := <[tM:=Excl (Push v)]> hsM.
-      set hs' := <[tM:=Excl (Push v)]> hs.
-      (* pure assertions to close AU *)
-      iDestruct (own_valid_2 with "Hh● Hh◯") as %Hincl'%frac_auth_included_total.
-      assert (stack_hist_cont hsM' = Some (v :: zs)) as Hcont' by by apply stack_hist_cont_push.
-      assert (∀ t' : nat, t' ∈ dom (gset nat) hs → t' < tM).
-      { inversion Hg as [_ Hdom_hsM]. apply (dom_included hs hsM) in Hincl. intros t' Ht'.
-        rewrite ->(elem_of_subseteq) in Hincl. specialize (Hincl t' Ht'). apply Hdom_hsM in Hincl. lia. }
-      iMod ("HClose" with "[Hs◯ Hh◯]") as "HΦ".
-      iFrame. iPureIntro. split; [by exists hsM', (S tM) | done].
-      iModIntro. iSplitR "HΦ". (* TODO: cleanup *)
-      + iModIntro. iExists hsM', (S tM), (v::zs). iFrame "∗ %". iExists (Some r). iFrame. simpl.
-        iExists w. iFrame. iExists 1%Qp. iFrame.
-      + by wp_pures.
+      iMod ("CloseAU" with "[Hh◯]") as "HΦ".
+      { assert (∀ t' : nat, t' ∈ dom (gset nat) hs → t' < tM).
+        inversion Hg as [_ Hdom_hsM]. apply (dom_included hs hsM) in Hincl. intros t' Ht'.
+        rewrite ->(elem_of_subseteq) in Hincl. specialize (Hincl t' Ht'). apply Hdom_hsM in Hincl. lia.
+        by iFrame "∗ %". }
+      iModIntro. iSplitR "HΦ". (* close the invariant *)
+      { iExists hsM', (S tM), (v::xs).
+        assert (stack_hist_cont hsM' = Some (v :: xs)) as Hcont' by by apply stack_hist_cont_push.
+        eauto 10 with iFrame. }
+      by wp_pures.
     - wp_cmpxchg_fail.
       { exact: not_inj. }
       { case u, w; simpl; eauto. }
-      iModIntro. iSplitL "Hs● Hh● Hl HPhys"; first by eauto 10 with iFrame.
+      iModIntro. iSplitL "Hh● Hl HPhys"; first by eauto 10 with iFrame.
       wp_pures. iApply "IH". iExact "AU".
   Qed.
 
-  Lemma pop_stack_spec (l : loc) (γs γh : gname) :
-    stack_hist γs γh l -∗
-    <<< ∀ xs q hs, stack_hist_snap γs γh q xs hs >>>
+  Lemma pop_stack_spec (l : loc) (γh : gname) :
+    stack_hist γh l -∗
+    <<< ∀ q hs, hist_snap γh q hs >>>
       pop_stack #l @ ⊤ ∖ ↑N
-    <<< match xs with
-        | [] => stack_hist_snap γs γh q [] hs
-        | v::xs' => ∃ (t:nat), stack_hist_snap γs γh q (xs') (<[t := Excl (Pop v)]> hs) ∗
-                 ⌜∀ (t':nat), t' ∈ (dom (gset nat) hs) → t' < t⌝
-        end,
+    <<< ∃ hsM xs,
+            (* TODO: the client should be able to know that hsM is the full history *)
+            ⌜hs ≼ hsM ∧ stack_hist_cont hsM = Some xs⌝ ∗
+            match xs with
+            | [] => hist_snap γh q hs
+            | v::_ => ∃ (t:nat), hist_snap γh q (<[t := Excl (Pop v)]> hs) ∗
+                             ⌜∀ (t':nat), t' ∈ (dom (gset nat) hs) → t' < t⌝
+            end,
         RET match xs with
             | [] => NONEV
             | v::_ => SOMEV v
             end >>>.
   Proof.
     iIntros "#SH" (Φ) "AU". iLöb as "IH". wp_lam. wp_bind (! _)%E.
-    iInv "SH" as (hsM tM xs) ">(HPhys & Hs● & Hh● & %)". rename H0 into Hcont.
+    iInv "SH" as (hsM tM xs) ">(HPhys & Hh● & %)". rename H0 into Hcont.
     iDestruct "HPhys" as (w) "[Hl HPhys]".
     wp_load.
     iDestruct (phys_list_dup with "HPhys") as "[HPhys1 HPhys2]".
     destruct w as [w|], xs as [|x xs]; try done; simpl.
     - (* non-empty stack *)
-      iModIntro. iSplitL "Hl Hs● Hh● HPhys1"; first by eauto 10 with iFrame.
+      iModIntro. iSplitL "Hl Hh● HPhys1". iExists hsM, tM, (x::xs). by eauto 10 with iFrame.
       clear Hcont hsM tM.
       wp_let. wp_match. iDestruct "HPhys2" as (r wq) "[Hw HP]".
       wp_load. wp_let. wp_proj. wp_bind (CmpXchg _ _ _)%E.
-      iInv "SH" as (hsM tM ys) ">(HPhys & Hs● & Hh● & %)". rename H0 into Hcont.
+      iInv "SH" as (hsM tM ys) ">(HPhys & Hh● & %)". rename H0 into Hcont.
       iDestruct "HPhys" as (u) "[Hl HPhys]".
       iClear "HP". clear xs.
       destruct (decide (u = Some w)) as [[= ->]|Hx].
       + wp_cmpxchg_suc.
         destruct ys; first done.
-        iMod "AU" as (zs q hs) "[(Hs◯ & Hh◯ & %) [_ HClose]]". rename H0 into Hcont_frag.
+        iMod "AU" as (q hs) "[Hh◯ [_ CloseAU]]".
 
         (* TODO: extracting pure stuff *)
         iDestruct "Hh●" as "[Hh● Hg]". iDestruct "Hg" as %Hg.
@@ -219,47 +197,39 @@ Section spec.
         iDestruct (own_valid_2 with "Hh● Hh◯") as %Hincl%frac_auth_included_total.
         iCombine "Hh●" "Hg" as "Hh●". iClear "Hg".
 
-        iDestruct (auth_agree with "Hs● Hs◯") as %<-.
-        iMod (auth_update γs ys with "Hs● Hs◯") as "[Hs● Hs◯]".
         iDestruct "HPhys" as (u wq') "[Hw' HPhys]".
         iDestruct (mapsto_agree with "Hw Hw'") as %[=-> ->%to_val_inj].
 
         iMod (hist_update γh q hsM hs tM (Pop v) with "Hh● Hh◯") as "[Hh● Hh◯]".
         iDestruct "Hh●" as "[Hh● %]". rename H0 into Hg'.
         set hsM' := <[tM:=Excl (Pop v)]> hsM.
-        set hs' := <[tM:=Excl (Pop v)]> hs.
-
-        (* pure assertions to close AU *)
-        rewrite /stack_hist_snap /hist /hist_snap /stack_cont.
-        iDestruct (own_valid_2 with "Hh● Hh◯") as %Hincl'%frac_auth_included_total.
-        assert (stack_hist_cont hsM' = Some ys) as Hcont' by by apply stack_hist_cont_pop.
-        assert (∀ t' : nat, t' ∈ dom (gset nat) hs → t' < tM).
-        { inversion Hg as [_ Hdom_hsM]. apply (dom_included hs hsM) in Hincl. intros t' Ht'.
-          rewrite ->(elem_of_subseteq) in Hincl. specialize (Hincl t' Ht'). apply Hdom_hsM in Hincl. lia. }
-
-        iMod ("HClose" with "[Hs◯ Hh◯]") as "HΦ".
-        iExists tM. iFrame. iPureIntro. split; [by exists hsM', (S tM) | done].
-        iModIntro. iSplitR "HΦ". (* TODO: cleanup *)
-        * iModIntro. iExists hsM', (S tM), ys. iFrame "∗ %". unfold phys_stack. iExists u. iFrame.
-        * by wp_pures.
+        iMod ("CloseAU" $! hsM (v::ys) with "[Hh◯]") as "HΦ".
+        { assert (∀ t' : nat, t' ∈ dom (gset nat) hs → t' < tM).
+          inversion Hg as [_ Hdom_hsM]. apply (dom_included hs hsM) in Hincl. intros t' Ht'.
+          rewrite ->(elem_of_subseteq) in Hincl. specialize (Hincl t' Ht'). apply Hdom_hsM in Hincl. lia.
+          eauto with iFrame. }
+        iModIntro. iSplitR "HΦ". (* close the invariant *)
+        { iExists hsM', (S tM), ys.
+          assert (stack_hist_cont hsM' = Some ys) as Hcont' by by apply stack_hist_cont_pop.
+          eauto 10 with iFrame. }
+        by wp_pures.
       + wp_cmpxchg_fail.
         { intro Heq. apply Hx. destruct u; inversion Heq; done. }
         iModIntro. iSplitR "AU"; first by eauto 10 with iFrame.
         wp_pures. iApply "IH". iExact "AU".
     - (* empty stack *)
       iClear "HPhys1 HPhys2".
-      iMod "AU" as (zs q hs) "[(Hs◯ & Hh◯ & %) [_ HClose]]". rename H0 into Hcont_frag. (* TODO: Hcont_frag not needed? *)
+      iMod "AU" as (q hs) "[Hh◯ [_ CloseAU]]".
       (* TODO: extracting pure stuff *)
       iDestruct "Hh●" as "[Hh● Hg]". iDestruct "Hg" as %Hg.
       iAssert (⌜hist_gapless tM hsM⌝)%I as "Hg"; first done.
       iDestruct (own_valid_2 with "Hh● Hh◯") as %Hincl%frac_auth_included_total.
       iCombine "Hh●" "Hg" as "Hh●". iClear "Hg".
 
-      iDestruct (auth_agree with "Hs● Hs◯") as %<-.
-      iMod ("HClose" with "[Hs◯ Hh◯]") as "HΦ".
-      { iFrame. by iExists hsM, tM. }
-      iModIntro. iSplitR "HΦ"; first by eauto 10 with iFrame.
-      wp_pures. iExact "HΦ".
+      iMod ("CloseAU" $! hsM [] with "[Hh◯]") as "HΦ"; first by eauto with iFrame.
+      iModIntro. iSplitR "HΦ".
+      { iExists hsM, tM, []. eauto with iFrame. }
+      by wp_pures.
   Qed.
 
 End spec.
